backend/LineartypingC.v
@@ -1,0 +1,134 @@
+Require Import CoqlibC.
+Require Import ASTC.
+Require Import Integers.
+Require Import ValuesC.
+Require Import GlobalenvsC.
+Require Import Memory.
+Require Import Events.
+Require Import Op.
+Require Import Machregs.
+Require Import LocationsC.
+Require Import Conventions.
+Require Import LTL.
+Require Import Linear.
+Require Import sflib.
+(** newly added **)
+Require Export Lineartyping.
+Require SoundTop.
+Require Import Preservation.
+Require Import ModSem.
+Require Import LinearC.
+
+Set Implicit Arguments.
+
+
+
+Lemma ls_init_has_type
+      ls_init sg vs
+      (LEN: length vs = length sg)
+      ir fr ofs
+      (LOCSET: typify_list vs sg = map (fun p => Locmap.getpair p ls_init) (loc_arguments_64 sg ir fr ofs))
+      sl pos ty
+      (IN: In (S sl pos ty) (regs_of_rpairs (loc_arguments_64 sg ir fr ofs)))
+      (ONES: forall lp, In lp (loc_arguments_64 sg ir fr ofs) -> is_one lp)
+  :
+    <<TY: Val.has_type (ls_init (S sl pos ty)) ty>>
+.
+Proof.
+  remember (loc_arguments_64 sg ir fr ofs) as locs in *.
+  Local Opaque Z.add Z.mul Z.sub Z.div.
+  Local Opaque loc_arguments_64.
+  ginduction locs; ii; ss. destruct vs; ss. destruct sg; ss. clarify.
+  unfold typify_list in *.
+  exploit ONES; eauto. i. destruct a; ss.
+  clarify.
+  des; cycle 1.
+  - Local Transparent loc_arguments_64.
+    ss. des_ifs; eapply IHlocs; eauto.
+  - clarify. rewrite <- H3.
+    assert(t = ty).
+    { clear - Heqlocs. ss. des_ifs. }
+    clarify.
+    eapply typify_has_type.
+Qed.
+
+
+Section SOUNDNESS.
+
+  Variable prog: program.
+
+  Hypothesis wt_prog:
+    forall i fd, In (i, Gfun fd) prog.(prog_defs) -> wt_fundef fd
+  .
+
+  Lemma mreg_type_any
+        mr
+    :
+      <<ANY: mreg_type mr = Tany64>>
+  .
+  Proof.
+    unfold mreg_type. des_ifs.
+  Qed.
+
+  Lemma has_type_any
+        v
+    :
+      <<ANY: Val.has_type v Tany64>>
+  .
+  Proof.
+    destruct v; ss.
+  Qed.
+
+  Theorem wt_state_local_preservation
+          skenv_link
+    :
+      local_preservation (modsem skenv_link prog) (fun _ _ st => wt_state st)
+  .
+  Proof.
+    econs; ii; ss; eauto.
+    - (* init *)
+      inv INIT.
+      assert(WTLS: wt_locset ls_init).
+      { ii.
+        destruct l; ss.
+        { rewrite mreg_type_any. apply has_type_any. }
+        destruct (classic (In (S sl pos ty) (regs_of_rpairs (loc_arguments (fn_sig fd))))).
+        - clear - LOCSET H LEN.
+          abstr (fn_sig fd) sg.
+          abstr (Args.vs args) vs. clear_tac.
+          generalize (loc_arguments_one sg). intro ONES.
+          destruct sg; ss. unfold loc_arguments in *. ss. des_ifs. clear_tac.
+          eapply ls_init_has_type; eauto.
+        - erewrite SLOT; eauto.
+      }
+      econs; eauto.
+      econs; eauto.
+      econs; eauto.
+    - inv STEP.
+      eapply step_type_preservation; eauto.
+      ii. unfold Genv.find_funct, Genv.find_funct_ptr in *. des_ifs.
+      unfold Skeleton.SkEnv.revive in *.
+      eapply Genv_map_defs_def in Heq. des. u in MAP. des_ifs_safe. bsimpl.
+      esplits. eapply in_prog_defmap; eauto.
+    - esplits; eauto.
+      ii.
+      inv AFTER.
+      inv SUST.
+      econs; eauto.
+      { destruct stack; ss.
+        des_ifs. inv WTSTK.
+        econs; eauto.
+        unfold locset_after_external. repeat intro. destruct l; eauto.
+        + destruct (is_callee_save r) eqn:T; eauto; simpl; eauto.
+        + destruct sl; eauto; simpl; eauto.
+      }
+      apply wt_setpair; auto.
+      { eapply typify_has_type; eauto. }
+      ii.
+      unfold locset_after_external. repeat intro. destruct l; eauto.
+      + destruct (is_callee_save r) eqn:T; eauto; simpl; eauto.
+      + destruct sl; eauto; simpl; eauto.
+  Qed.
+
+End SOUNDNESS.
+
