x86/Conventions1C.v
@@ -1,0 +1,30 @@
+Require Import CoqlibC Decidableplus.
+Require Import ASTC Machregs Locations.
+(** newly added **)
+Require Export Conventions1.
+
+Set Implicit Arguments.
+
+
+
+Lemma loc_arguments_length_aux
+      tys ir fr ofs
+  :
+    <<LEN: length (loc_arguments_64 tys ir fr ofs) = length tys>>
+.
+Proof.
+  ginduction tys; ii; ss.
+  des_ifs; s; rewrite IHtys; ss.
+Qed.
+
+Lemma loc_arguments_length
+      sg
+  :
+    <<LEN: length (loc_arguments sg) = length (sig_args sg)>>
+.
+Proof.
+  destruct sg; ss.
+  unfold loc_arguments. des_ifs. ss.
+  rewrite loc_arguments_length_aux. ss.
+Qed.
+
